src/example/LockClientSC.v
@@ -1,0 +1,94 @@
+From sflib Require Import sflib.
+From Paco Require Import paco.
+Require Import Coq.Classes.RelationClasses Lia Program.
+Unset Universe Checking.
+
+From Fairness Require Export
+     ITreeLib WFLib FairBeh NatStructs Mod pind Axioms
+     OpenMod SCM Red IRed Wrapper WeakestAdequacy FairLock Concurrency.
+From Ordinal Require Export ClassicalHessenberg.
+
+Set Implicit Arguments.
+
+
+Module ClientImpl.
+  Definition loc_X := SCMem.val_ptr (0, 0).
+
+  Definition const_0 := SCMem.val_nat 0.
+  Definition const_42 := SCMem.val_nat 42.
+
+  Definition thread1:
+    ktree ((((@eventE void) +' cE) +' (sE unit)) +' OpenMod.callE) unit unit
+    :=
+    fun _ =>
+      `_: unit <- (OMod.call "lock" tt);;
+      `_: unit <- (OMod.call "store" (loc_X, const_42));;
+      `_: unit <- (OMod.call "unlock" tt);;
+      Ret tt.
+
+  Definition thread2:
+    ktree ((((@eventE void) +' cE) +' (sE unit)) +' OpenMod.callE) unit unit
+    :=
+    fun _ =>
+      _ <- ITree.iter
+            (fun (_: unit) =>
+               `_: unit <- (OMod.call "lock" tt);;
+               x <- (OMod.call "load" loc_X);;
+               `_: unit <- (OMod.call "unlock" tt);;
+               b <- OMod.call "compare" (x: SCMem.val, SCMem.val_nat 0);;
+               if (b: bool) then Ret (inl tt) else Ret (inr tt)) tt;;
+      x <- (OMod.call "load" loc_X);;
+      match x with
+      | SCMem.val_nat n => _ <- trigger (Observe 0 [n]);; Ret tt
+      | _ => UB
+      end.
+
+  Definition omod: OMod.t :=
+    OMod.mk
+      tt
+      (Mod.get_funs [("thread1", Mod.wrap_fun thread1);
+                     ("thread2", Mod.wrap_fun thread2)])
+  .
+
+  Definition mod: Mod.t :=
+    OMod.close
+      (omod)
+      (ModAdd WMem.mod FairLockW.mod)
+  .
+
+End ClientImpl.
+
+
+Module ClientSpec.
+  Definition thread1:
+    ktree ((((@eventE void) +' cE) +' (sE unit))) unit unit
+    :=
+    fun _ =>
+      Ret tt.
+
+  Definition thread2:
+    ktree ((((@eventE void) +' cE) +' (sE unit))) unit unit
+    :=
+    fun _ =>
+      _ <- trigger (Observe 0 [42]);;
+      Ret tt.
+
+  Definition mod: Mod.t :=
+    Mod.mk
+      tt
+      (Mod.get_funs [("thread1", Mod.wrap_fun thread1);
+                     ("thread2", Mod.wrap_fun thread2)])
+  .
+
+End ClientSpec.
+
+
+From Fairness Require Import ModSim.
+
+Section SIM.
+  Let config := [("thread1", tt↑); ("thread2", tt↑)].
+
+  Lemma client_correct:
+    UserSim.sim ClientSpec.mod ClientImpl.mod (prog2ths ClientSpec.mod config) (prog2ths ClientImpl.mod config).
+  Admitted.
+End SIM.
