src/logic/Weakest.v
@@ -1634,37 +1634,37 @@ Section STATE.
   Qed.
 
   (* TODO *)
-  Lemma stsim_yieldR0 E r g R_src R_tgt
-        (Q: R_src -> R_tgt -> iProp)
-        ktr_src ktr_tgt l
-    :
-    (ObligationRA.duty (inl tid) l ∗ ObligationRA.tax l)
-      -∗
-      ((ObligationRA.duty (inl tid) l)
-         -∗
-         (MUpd (nth_default True%I Invs) E topset
-               ((FairRA.white_thread (_Id:=_))
-                  -∗
-                  (stsim topset r g Q (trigger (Yield) >>= ktr_src) (ktr_tgt tt))))
-      )
-      -∗
-      (stsim E r g Q (trigger (Yield) >>= ktr_src) (trigger (Yield) >>= ktr_tgt))
-  .
-  Proof.
-    iIntros "H K".
-    unfold stsim. iIntros (? ? ? ? ?) "[D C]".
-    iApply isim_yieldR. unfold I. iFrame.
-    iPoseProof "H" as "[DUTY TAX]".
-    iPoseProof ("K" with "DUTY C") as "K".
-    iPoseProof "K" as "> K".
-    unfold MUpd. iPoseProof ("K" with "C") as "[C K]".
-    iIntros (? ? ? ? ? ?) "[D C] %".
-    iPoseProof ("H" with "C") as "> K". iDestruct "K" as (l) "[DX K]".
-    iPoseProof (default_I_update_ident_thread with "D DX") as "> [[DUTY WHITE] D]".
-    { eauto. }
-    iPoseProof ("K" with "DUTY WHITE") as "[IV K]".
-    iApply "K". iFrame.
-  Qed.
+  (* Lemma stsim_yieldR0 E r g R_src R_tgt *)
+  (*       (Q: R_src -> R_tgt -> iProp) *)
+  (*       ktr_src ktr_tgt l *)
+  (*   : *)
+  (*   (ObligationRA.duty (inl tid) l ∗ ObligationRA.tax l) *)
+  (*     -∗ *)
+  (*     ((ObligationRA.duty (inl tid) l) *)
+  (*        -∗ *)
+  (*        (MUpd (nth_default True%I Invs) E topset *)
+  (*              ((FairRA.white_thread (_Id:=_)) *)
+  (*                 -∗ *)
+  (*                 (stsim topset r g Q (trigger (Yield) >>= ktr_src) (ktr_tgt tt)))) *)
+  (*     ) *)
+  (*     -∗ *)
+  (*     (stsim E r g Q (trigger (Yield) >>= ktr_src) (trigger (Yield) >>= ktr_tgt)) *)
+  (* . *)
+  (* Proof. *)
+  (*   iIntros "H K". *)
+  (*   unfold stsim. iIntros (? ? ? ? ?) "[D C]". *)
+  (*   iApply isim_yieldR. unfold I. iFrame. *)
+  (*   iPoseProof "H" as "[DUTY TAX]". *)
+  (*   iPoseProof ("K" with "DUTY C") as "K". *)
+  (*   iPoseProof "K" as "> K". *)
+  (*   unfold MUpd. iPoseProof ("K" with "C") as "[C K]". *)
+  (*   iIntros (? ? ? ? ? ?) "[D C] %". *)
+  (*   iPoseProof ("H" with "C") as "> K". iDestruct "K" as (l) "[DX K]". *)
+  (*   iPoseProof (default_I_update_ident_thread with "D DX") as "> [[DUTY WHITE] D]". *)
+  (*   { eauto. } *)
+  (*   iPoseProof ("K" with "DUTY WHITE") as "[IV K]". *)
+  (*   iApply "K". iFrame. *)
+  (* Qed. *)
 
   Lemma stsim_sync E r g R_src R_tgt
         (Q: R_src -> R_tgt -> iProp)
